theories/Effects/StateFacts.v
@@ -63,14 +63,14 @@ Instance eq_itree_interp_state {E F S R} (h : E ~> Monads.stateT S (itree F)) :
          (interp_state h R).
 Proof.
   revert_until R.
-  ucofix CIH. intros h x y H0 x2 y0 H1.
+  wcofix CIH. intros h x y H0 x2 y0 H1.
   rewrite !unfold_interp_state.
   unfold _interp_state.
-  uunfold H0; repeat red in H0.
+  wunfold H0; repeat red in H0.
   genobs x ox; destruct ox; simpobs; dependent destruction H0; simpobs; subst.
-  - constructor. eauto.
-  - constructor. eauto with paco.
-  - constructor. uclo eq_itree_clo_bind. econstructor.
+  - wstep. constructor. eauto.
+  - wstep. constructor. eauto with paco.
+  - wstep. constructor. wclo eq_itree_clo_bind. econstructor.
     + reflexivity.
     + intros [] _ []. auto with paco.
 Qed.
@@ -119,7 +119,7 @@ Lemma interp_state_bind {E F : Type -> Type} {A B S : Type}
   (interp_state f _ t s >>= fun st => interp_state f _ (k (snd st)) (fst st)).
 Proof.
   revert A t k s.
-  ucofix CIH.
+  wcofix CIH.
   intros A t k s.
   rewrite unfold_bind, (unfold_interp_state f t).
   destruct (observe t).
@@ -127,10 +127,10 @@ Proof.
   - cbn. rewrite !bind_ret. simpl.
     apply reflexivity.
   - cbn. rewrite !bind_tau, interp_state_tau.
-    econstructor. ubase. apply CIH.
+    wstep. econstructor. wbase. apply CIH.
   - cbn. rewrite interp_state_vis, bind_tau, bind_bind.
-    constructor.
-    uclo eq_itree_clo_bind. econstructor.
+    wstep. constructor.
+    wclo eq_itree_clo_bind. econstructor.
     + reflexivity.
     + intros u2 ? []. specialize (CIH _ (k0 (snd u2)) k (fst u2)).
       auto with paco.
@@ -141,19 +141,19 @@ Instance eutt_interp_state {E F: Type -> Type} {S : Type}
   Proper (eutt eq ==> eq ==> eutt eq) (@interp_state E (itree F) S _ _ _ h R).
 Proof.
   repeat intro. subst. revert_until R.
-  ucofix CIH. red. ucofix CIH'. intros.
+  wcofix CIH. wstep. wcofix CIH'. intros.
 
-  rewrite !unfold_interp_state. do 2 uunfold H0.
+  rewrite !unfold_interp_state. do 2 wunfold H0.
   induction H0; intros; subst; simpl.
-  - constructor. eauto.
-  - constructor.
-    uclo eutt0_clo_bind; econstructor; [reflexivity|].
+  - wstep. constructor. eauto.
+  - wstep. constructor.
+    wclo eutt0_clo_bind; econstructor; [reflexivity|].
     intros; subst.
-    ubase. eapply CIH'. edestruct EUTTK; eauto with paco.
-  - econstructor. eauto 9 with paco.
-  - constructor. eutt0_fold.
+    wbase. eapply CIH'. edestruct EUTTK; eauto with paco.
+  - wstep. econstructor. eauto 9 with paco.
+  - apply eutt0_tau_left.
     rewrite unfold_interp_state; auto.
-  - constructor. eutt0_fold.
+  - apply eutt0_tau_right.
     rewrite unfold_interp_state; auto.
 Qed.
 
@@ -169,13 +169,13 @@ Lemma interp_state_loop {E F S A B C} (RS : S -> S -> Prop)
           (interp_state h B (loop_ t1 ca) s1)
           (interp_state h B (loop_ t2 ca) s2)).
 Proof.
-  ucofix CIH. red. ucofix CIH'. intros.
+  wcofix CIH. wstep. wcofix CIH'. intros.
 
   rewrite (itree_eta (loop_ t1 ca)), (itree_eta (loop_ t2 ca)), !unfold_loop''.
   unfold loop_once. rewrite <- !itree_eta, !interp_state_bind.
-  uclo eutt0_clo_bind. econstructor; eauto.
+  wclo eutt0_clo_bind. econstructor; eauto.
   intros. destruct RELv. rewrite H2. destruct (snd v2).
   - rewrite !interp_state_tau.
-    econstructor. eauto with paco.
-  - rewrite !interp_state_ret. econstructor. eauto.
+    wstep. econstructor. eauto with paco.
+  - rewrite !interp_state_ret. wstep. econstructor. eauto.
 Qed.
